

Mahati Gorthy

HW#6

1. 4 Prove or give a counterexample: If  $V$  is finite-dimensional and  $U$  is a subspace of  $V$  that is invariant under every operator on  $V$ , then  $U = \{0\}$  or  $U = V$ .

when we say invariant under every operator, we mean that for every  $T: V \rightarrow V$ ,  $T(U) \subseteq U$

let's suppose  $U \neq \{0\}$  and  $U \neq V$  which means we can choose some  $u \in U$  with  $u \neq 0$  and there is some vector  $v \in V$  with  $v \notin U$

using Thm 3.10 { now if we build some operator  $T: V \rightarrow V$  such that  $T(u) = v$   
for all other basis vectors, we can let  $T$  send it to 0

since  $u \in U$  but  $T(u) = v \notin U$ , using  $T$  moves a vector from  $U$  to outside of  $U$

but if  $U$  is invariant under every operator, it should be the case that  $T(u) \in U$  for all  $T$  which leads to a contradiction

thus no nonzero subspace can be invariant under every operator, only  $U = \{0\}$  and  $U = V$  works

2. 7 Define  $T \in \mathcal{L}(\mathbb{F}^3)$  by  $T(z_1, z_2, z_3) = (2z_2, 0, 5z_3)$ . Find all eigenvalues and eigenvectors of  $T$ .

$$T(z_1, z_2, z_3) = \lambda(z_1, z_2, z_3)$$

$$\text{we can say } 2z_2 = \lambda z_1 \quad 0 = \lambda z_2 \quad 5z_3 = \lambda z_3$$

$$\text{case 1: } \lambda = 5 \quad \text{from } 0 = \lambda z_2 \text{ with } \lambda \neq 0, \text{ we get } z_2 = 0$$

$$\text{from } 2z_2 = \lambda z_1, \text{ we get } 0 = 5z_1, \text{ thus } z_1 = 0$$

$$5z_3 = 5z_3 \rightarrow z_3 \text{ is free and must be nonzero for an eigenvector}$$

$$\text{thus } \{(0, 0, z_3) : z_3 \in \mathbb{F}\} = \text{span}\{(0, 0, 1)\}$$

$$\text{case 2: } \lambda = 0 \quad \text{we get } 2z_2 = 0 \quad 0 = 0 \quad 5z_3 = 0 \quad \text{which forces } z_2 = 0 \text{ and } z_3 = 0$$

$$\text{thus } \{(z_1, 0, 0) : z_1 \in \mathbb{F}\} = \text{span}\{(1, 0, 0)\}$$

and final  
eigenvalues:  $\lambda = 0, 5$

3. 15 Suppose  $V$  is finite-dimensional,  $T \in \mathcal{L}(V)$ , and  $\lambda \in F$ . Show that  $\lambda$  is an eigenvalue of  $T$  if and only if  $\lambda$  is an eigenvalue of the dual operator  $T' \in \mathcal{L}(V')$ .

we're assuming that  $V$  is fin. dim.,  $T \in \mathcal{L}(V)$  and  $\lambda \in F$

we're also letting  $T' \in \mathcal{L}(V')$  be the dual operator and we define it as  $T'(\phi) = \phi \circ T$  for all  $\phi \in V'$

we know these definitions:

$\lambda$  is an eigenvalue of  $T$  if there exists a nonzero vector  $v \in V$  such that  $T(v) = \lambda v$

$\lambda$  is an eigenvalue of  $T'$  if there exists a nonzero  $\phi \in V'$  such that  $T'(\phi) = \lambda \phi$  which means for all  $v \in V$ ,

$$T'(\phi)(v) = \lambda \phi(v) \text{ but since } T'(\phi) = \phi \circ T, \text{ we're basically saying } \phi(Tv) = \lambda \phi(v) \text{ for all } v \in V$$

let's first prove  $(\Rightarrow)$

we're assuming  $\lambda$  is an eigenvalue of  $T$

if  $\lambda$  is an eigenvalue of  $T$ , then there exists a nonzero  $v \in V$  s.t.  $T(v) = \lambda v$

now, if we take any  $\phi \in V'$ , we know that  $T'(\phi) = \phi \circ T$

then for any  $v \in V$ , we have  $T'(\phi)(v) = (\phi \circ T)(v) = \phi(Tv)$

and specifically for our eigenvector  $v$ ,

$$T'(\phi)(v) = \phi(Tv) = \phi(\lambda v) = \lambda \phi(v)$$

This shows that  $T'$  on any  $\phi$  at  $v$  scales  $\phi(v)$  by  $\lambda$

and thus  $\lambda$  is an eigenvalue of  $T'$  corresponding to  $\phi$

now  $(\Leftarrow)$  we're assuming  $\lambda$  is an eigenvalue of  $T'$

then, there exists some nonzero  $\phi \in V'$  such that  $T'(\phi) = \lambda \phi$

by def. of  $T'$ , this means that for every  $v \in V$ ,

$$T'(\phi)(v) = \phi(Tv) = \lambda \phi(v)$$

and we can say  $\phi(Tv - \lambda v) = 0$  for all  $v \in V$

this means that every vector  $Tv - \lambda v$  is sent to 0 by  $\phi$  → nullspace of  $\phi$

↳ if we say that  $\lambda$  is not an eigenvalue of  $T$  that would mean for every  $v \in V$ ,

there is a  $v$  such that  $w = Tv - \lambda v$ , so every vector in  $V$  is in the null space of  $\phi$

but if a functional is zero on all  $V$ , then it must be the zero functional

which leads to a contradiction because we assumed  $\phi$  is nonzero

thus  $\lambda$  must be an eigenvalue of  $T$

4.

16 Suppose  $v_1, \dots, v_n$  is a basis of  $V$  and  $T \in \mathcal{L}(V)$ . Prove that if  $\lambda$  is an eigenvalue of  $T$ , then

$$|\lambda| \leq n \max\{|\mathcal{M}(T)_{j,k}| : 1 \leq j, k \leq n\},$$

where  $\mathcal{M}(T)_{j,k}$  denotes the entry in row  $j$ , column  $k$  of the matrix of  $T$  with respect to the basis  $v_1, \dots, v_n$ .

See Exercise 19 in Section 6A for a different bound on  $|\lambda|$ .

we're assuming that  $v_1, \dots, v_n$  is a basis of  $V$  and  $T \in \mathcal{L}(V)$  and  $\lambda$  is an eigenvalue of  $T$

we can let  $M(T)$  be the  $n \times n$  matrix of  $T$  with respect to the basis  $v_1, \dots, v_n$

the entries of this are  $M(T)_{j,k}$

$$\text{this means that } T(v_k) = \sum_{j=1}^n M(T)_{j,k} v_j$$

if we say  $\lambda$  is an eigenvalue of  $T$ , then there exists a nonzero vector  $v \in V$  such that  $T(v) = \lambda v$

since  $v_1, \dots, v_n$  is a basis, we can write  $v$  as a linear combination of the

basis vectors:  $v = c_1 v_1 + \dots + c_n v_n$  where not all  $c_k$  are 0

$$\text{then if we do } T(v) = T\left(\sum_{k=1}^n c_k v_k\right) = \sum_{k=1}^n c_k T(v_k)$$

and if we substitute  $T(v_k)$  with the matrix entries

$$T(v) = \sum_{k=1}^n c_k \left( \sum_{j=1}^n M(T)_{j,k} v_j \right) = \sum_{j=1}^n \left( \sum_{k=1}^n M(T)_{j,k} c_k \right) v_j$$

we also can say

$$T(v) = \lambda v = \lambda \sum_{j=1}^n c_j v_j = \sum_{j=1}^n (\lambda c_j) v_j$$

since  $v_1, \dots, v_n$  is a basis, the coefficients of the lin. combinations must be equal

$$\text{comparing } v_j \text{ in both, we get } \lambda c_j = \sum_{k=1}^n M(T)_{j,k} c_k \text{ for each } j=1, \dots, n$$

well this is the eigenvalue equation in matrix form:  $M(T)c = \lambda c$  where  $c$  is the column vector of the coefficients  $\begin{bmatrix} c_1 \\ \vdots \\ c_n \end{bmatrix}$

if we let  $c_p$  be a coefficient with the largest abs. value among all the coefficients of  $v$ ,

so basically  $|c_p| = \max\{|c_1|, \dots, |c_n|\}$  <sup>and</sup> since  $v$  is a non zero vector  $|c_p| > 0$

so if we look at equation for row  $p$ :  $\lambda c_p = \sum_{k=1}^n M(T)_{p,k} c_k$  and take abs. value of both sides and use Triangle Inequality, we get

$$|\lambda c_p| = \left| \sum_{k=1}^n M(T)_{p,k} c_k \right| \leq \sum_{k=1}^n |M(T)_{p,k} c_k| = \sum_{k=1}^n |M(T)_{p,k}| |c_k|$$

then if we let  $M = \max \{ |M(T)_{j,k}| : 1 \leq j, k \leq n \}$

we can use the fact that  $|c_k| \leq |c_p|$  for all  $k$ , and  $|M(T)_{p,k}| \leq M$  for all  $k$ , and say

$$\sum_{k=1}^n |M(T)_{p,k}| |c_k| \leq \sum_{k=1}^n M |c_p| = M |c_p| \sum_{k=1}^n 1 = n M |c_p|$$

so we get  $|\lambda c_p| \leq n M |c_p|$

since  $|c_p| > 0$ , we can divide both sides by  $|c_p|$  to get  $|\lambda| \leq n M$

and if we substitute to def. of  $M$ , we get  $|\lambda| \leq n \max \{ |M(T)_{j,k}| : 1 \leq j, k \leq n \}$

5. 19 Show that the forward shift operator  $T \in \mathcal{L}(F^\infty)$  defined by

$$T(z_1, z_2, \dots) = (0, z_1, z_2, \dots)$$

has no eigenvalues.

we're saying  $T \in \mathcal{L}(F^\infty)$  and  $T(z_1, z_2, z_3, \dots) = (0, z_1, z_2, z_3, \dots)$

let's assume that there exists a scalar  $\lambda$  and a non-zero vector  $z = (z_1, z_2, z_3, \dots)$  such that  $Tz = \lambda z$

then using the eigenvalue equation:

$$T(z_1, z_2, z_3, \dots) = \lambda(z_1, z_2, z_3, \dots)$$

$$(0, z_1, z_2, z_3, \dots) = (\lambda z_1, \lambda z_2, \lambda z_3, \dots)$$

$$\begin{aligned} \text{if we do this, we get } 0 &= \lambda z_1 \\ z_1 &= \lambda z_2 \\ z_2 &= \lambda z_3 \\ &\vdots \end{aligned}$$

there are two cases:

case 1:  $\lambda = 0$  if  $\lambda = 0$ , then with the first equation,  $0 = \lambda z_1$  is trivially satisfied

the rest of the equations become

$$z_1 = 0 \cdot z_2 = 0$$

$$z_2 = 0 \cdot z_3 = 0$$

$\vdots$

which implies that  $z_1 = z_2 = z_3 = \dots = 0$

so the only eigenvector corresponding to  $\lambda = 0$  is  $z = (0, 0, \dots)$  but by def. an eigenvector must not be  $\emptyset$  thus  $\lambda = 0$  is not an eigenvalue

case 2:  $\lambda \neq 0$

if  $\lambda \neq 0$ , then  $0 = \lambda z_1 \Rightarrow$  it must be that  $z_1 = 0$

then  $z_1 = \lambda z_2 \Rightarrow 0 = \lambda z_2 \Rightarrow z_2 = 0 \dots$  and so

we can see that  $z_n = 0$  for all  $n \geq 1$  meaning the only eigenvector is  $z = (0, 0, \dots)$

but an eigenvector must not be  $\emptyset$

both cases lead to a contradiction, thus the forward shift operator has no eigenvalues

6. 39 Suppose  $V$  is finite-dimensional and  $T \in \mathcal{L}(V)$ . Prove that  $T$  has an eigenvalue if and only if there exists a subspace of  $V$  of dimension  $\dim V - 1$  that is invariant under  $T$ .

let's first prove ( $\Rightarrow$ ) if  $T$  has an eigenvalue, then the subspace exists

let  $\lambda \in F$  be an eigenvalue of  $T$

then there exists a nonzero vector  $v \in V$  such that  $T(v) = \lambda v$

we can make subspace  $U$  of  $\dim V - 1$  that is invariant under  $T$

since  $v \neq 0$ , we can extend  $\{v\}$  to be a basis of  $V$ :  $\{v, v_2, v_3, \dots, v_n\}$

then we can let  $U = \text{span}\{v_2, v_3, \dots, v_n\}$

then  $\dim U = n - 1 = \dim V - 1$

now we must show that  $T(U) \subseteq U$

we can take  $u \in U$

since  $\{v_1, v_2, \dots, v_n\}$  is a basis, we can say  $T(u) = a_1 v_1 + a_2 v_2 + \dots + a_n v_n$  for some  $a_i$  scalars

we must show that  $a_1 = 0$  meaning  $T(u)$  has no component in the  $v$  direction so it lies completely inside  $U$

we can define  $\phi \in V^*$  by  $\phi(v) = 1$   $\phi(v_j) = 0$  for all  $j \geq 2$

then for any  $w = b_1 v + \dots + b_n v_n$ ,  $\phi(w) = b_1$

now:  $(T'(\phi))(v) = \phi(Tv) = \phi(\lambda v) = \lambda \phi(v) = \lambda$

for any  $u \in U$   $(T'(\phi))(u) = \phi(Tu) = a_1$  but we can also do  $T'(\phi) = \lambda \phi$  from  $Tv = \lambda v$  which means

$(T'(\phi))(u) = \lambda \phi(u) = \lambda \cdot 0 = 0$  and thus  $a_1 = 0$

therefore  $T(u)$  has no  $v$ -component, so  $T(u) \in U$  and  $U$  is invariant under  $T$ , and  $\dim U = \dim V - 1$

proving ( $\Leftarrow$ )

let's assume there exists a subspace  $U \subseteq V$  such that  $\dim U = \underbrace{\dim V - 1}_n$  and  $T(U) \subseteq U$

we want to show that  $T$  has an eigenvalue

we can choose  $\{w_1, \dots, w_{n-1}\}$  for  $U$  and extend to a basis of  $V$   $\{w_1, \dots, w_{n-1}, v\}$

now:  $T(v) = u + cv$  where  $u \in U$  and  $c$  is a scalar

if we suppose  $T(v) = u + cv$

$\hookrightarrow$  if  $u \neq 0$  then  $(T - cI)(v) = u$

if  $c$  were not an eigenvalue, then  $T - cI$  on  $v$  would "enter" the subspace, contradicting direct sum definition

thus we can show that  $T$  has an eigenvalue

7. 10 Suppose  $V$  is finite-dimensional,  $T \in \mathcal{L}(V)$ , and  $v \in V$ . Prove that  
 $\text{span}(v, Tv, \dots, T^m v) = \text{span}(v, Tv, \dots, T^{\dim V - 1} v)$   
 for all integers  $m \geq \dim V - 1$ .

we're letting  $V$  be a fin. dim. vector space,  $T \in \mathcal{L}(V)$ , and  $v \in V$

let's let  $n = \dim V$

we can say  $S = (v, Tv, T^2 v, \dots, T^m v)$

$$A = \text{span}(v, \dots, T^m v)$$

$$B = \text{span}(v, \dots, T^{n-1} v)$$

we want to show that  $A = B$  for  $m \geq n-1$

in any  $n$ -dim. space, any set of more than  $n$  vectors is linearly dependent <sup>given earlier in textbook</sup>

so in the list  $v, Tv, \dots, T^n v$ , there must be a nontrivial linear comb. among the first  $n+1$  vectors:

$$a_0 v + a_1 Tv + \dots + a_n T^n v = 0 \quad \text{with not all } a_i \text{ zero}$$

thus  $T^n v$  can always be written as a lin. comb. of  $v, Tv, \dots, T^{n-1} v$

and by the same logic:

$T^{n+1} v$  is a comb. of previous vectors

so all higher powers add nothing new to the span

now we must show  $A \subseteq B$

any element in  $A$  can be written as a comb. of  $v, Tv, \dots, T^m v$

but for  $k \geq n$ , each  $T^k v$  can be written as a comb. of  $v, Tv, \dots, T^{n-1} v$  so there don't increase the span

thus  $A \subseteq B$

now we must show  $B \subseteq A$

since  $m \geq n-1$ , all basis vectors of  $B$  ( $v, \dots, T^{n-1} v$ ) are also in  $A$ . So, every element of  $B$  is in  $A$

thus  $A = B$

11 Suppose  $V$  is a two-dimensional vector space,  $T \in \mathcal{L}(V)$ , and the matrix of

$T$  with respect to some basis of  $V$  is  $\begin{pmatrix} a & c \\ b & d \end{pmatrix}$ .

- (a) Show that  $T^2 - (a+d)T + (ad-bc)I = 0$ .  
 (b) Show that the minimal polynomial of  $T$  equals

$$\begin{cases} z-a & \text{if } b=c=0 \text{ and } a=d, \\ z^2 - (a+d)z + (ad-bc) & \text{otherwise.} \end{cases}$$

(a) let's first compute  $T^2 = T \cdot T = \begin{pmatrix} a & c \\ b & d \end{pmatrix} \begin{pmatrix} a & c \\ b & d \end{pmatrix}$

$$T^2 = \begin{pmatrix} a^2+bc & c(a+d) \\ b(a+d) & d^2+bc \end{pmatrix}$$

now, we can compute  $T^2 - (a+d)T + (ad-bc)I$

$$(a+d)T = (a+d) \begin{pmatrix} a & c \\ b & d \end{pmatrix} = \begin{pmatrix} a(a+d) & c(a+d) \\ b(a+d) & d(a+d) \end{pmatrix}$$

$$(ad-bc)I = \begin{pmatrix} ad-bc & 0 \\ 0 & ad-bc \end{pmatrix}$$

now  $T^2 - (a+d)T + (ad-bc)I$

↳ and if we do these

$$\text{first entry: } (a^2+bc) - (a^2+ad) + (ad-bc) = 0$$

$$\text{second entry: } (c(a+d)) - (ac+cd) + 0 = 0$$

$$\text{bottom left: } (b(a+d)) - (ba+db) + 0 = 0$$

$$\text{bottom right: } (d^2+bc) - (ad+d^2) + (ad-bc) = 0$$

every entry is 0 thus  $T^2 - (a+d)T + (ad-bc)I = 0$

(b)  $m_T(z)$  is the monic polynomial of least degree such that  $m_T(T) = 0$

case 1:  $b=c=0$  and  $a=d$  then  $T = aI$

then  $T(v) = av$  for all  $v$

$$\text{if we try } p(z) = z-a \text{ then } p(T)(v) = (T-aI)(v) = T(v) - av = av - av = 0$$

this works for any vector  $v$ , and is of degree 1 and monic

there are no lower-degree polynomials that work so the minimal polynomial is  $z-a$

case 2: try degree 1:  $p(z) = z-r$  for any  $r \in \mathbb{F}$

$p(T) = T-rI$  if  $T \neq rI$  then there's at least one entry of  $T-rI$  that is not zero, so

$p(T)$  is not the zero operator

try degree 2: characteristic polynomial  $p(z) = z^2 - (a+d)z + (ad-bc)$

$$p(T) = T^2 - (a+d)T + (ad-bc)I$$

calculate  $p(T)$  as an operator:

$$\text{for any } v, \text{ do } T(T(v)) - (a+d)T(v) + (ad-bc)v$$

when do all calculations (from part (a)), we get 0

so the min. poly. must be degree 2  $m_T(z) = z^2 - (a+d)z + (ad-bc)$